Rework fresh, Improve Allocation infrastructure.

theories/Infra/Fresh.v
@@ -1,5 +1,6 @@
 Require Import CSet Le Arith.Compare_dec.
 Require Import Plus Util Map Get Take LengthEq SafeFirst.
+Require Export StableFresh.
 
 Set Implicit Arguments.
 
@@ -196,85 +197,6 @@ Qed.
 
 Hint Resolve fresh_list_length : len.
 
-Section FreshListStable.
-
-  Variable fresh : set nat -> nat -> nat.
-
-  Fixpoint fresh_list_stable (G:set nat) (xl:list nat) : list nat :=
-    match xl with
-      | nil => nil
-      | x::xl => let y := fresh G x in y::fresh_list_stable {y;G} xl
-    end.
-
-  Lemma fresh_list_stable_length (G:set nat) xl
-  : length (fresh_list_stable G xl) = length xl.
-  Proof.
-    general induction xl; eauto. simpl. f_equal; eauto.
-  Qed.
-
-  Hypothesis fresh_spec : forall G x, fresh G x ∉ G.
-
-  Definition fresh_set_stable (G:set nat) L : set nat :=
-    of_list (fresh_list_stable G L).
-
-  Lemma fresh_list_stable_spec
-    : forall (G:set nat) L, disj (of_list (fresh_list_stable G L)) G.
-  Proof.
-    intros. general induction L; simpl; intros; eauto.
-    - hnf; intros. cset_tac'.
-      + specialize (H ({fresh G a; G})).
-        eapply H; eauto.
-        cset_tac.
-  Qed.
-
-  Lemma fresh_set_stable_spec
-  : forall (G:set nat) L, disj (fresh_set_stable G L) G.
-  Proof.
-    unfold fresh_set. eapply fresh_list_stable_spec.
-  Qed.
-
-  Lemma fresh_list_stable_nodup (G: set nat) L
-    : NoDupA eq (fresh_list_stable G L).
-  Proof.
-    general induction L; simpl; eauto.
-    econstructor; eauto. intro.
-    eapply fresh_list_stable_spec.
-    eapply InA_in. eapply H.
-    cset_tac; eauto.
-  Qed.
-
-End FreshListStable.
-
-Lemma fresh_list_stable_ext n G G' f
-  : (forall x G G', G [=] G' -> f G x = f G' x)
-    -> G [=] G'
-    -> fresh_list_stable f G n = fresh_list_stable f G' n.
-Proof.
-  intros EXT EQ. general induction n; simpl.
-  - reflexivity.
-  - f_equal; eauto using least_fresh_ext.
-    eapply IHn; eauto.
-    erewrite EXT, EQ; eauto; reflexivity.
-Qed.
-
-Lemma fresh_list_stable_get (fresh : ⦃nat⦄ -> nat -> nat) (G: set nat) L x n
-      (fresh_ext: forall x G G', G [=] G' -> fresh G x = fresh G' x)
-  : NoDupA eq L
-    -> get (fresh_list_stable fresh G L) n x
-    -> exists y, get L n y /\
-           x = fresh (of_list (take n (fresh_list_stable fresh G L)) ∪ G) y.
-Proof.
-  intros ND Get. general induction ND; simpl in *.
-  - isabsurd.
-  - inv Get.
-    + simpl. erewrite fresh_ext; eauto.
-      eexists; split; eauto with get. clear; cset_tac.
-    + edestruct IHND; eauto; dcr; subst.
-      eexists; split; eauto using get.
-      simpl. eapply fresh_ext. clear; cset_tac.
-Qed.
-
-Hint Resolve fresh_list_stable_length : len.
 
 Lemma least_fresh_list_small G n
 : forall i x, get (fresh_list least_fresh G n) i x -> x < cardinal G + n.
@@ -363,11 +285,3 @@ Proof.
   eapply fresh_list_nodup, fresh_spec. eauto with len.
   eapply fresh_list_spec, fresh_spec.
 Qed.
-
-Record StableFresh :=
-  {
-    stable_fresh :> set nat -> nat -> nat;
-    stable_fresh_spec : forall G x, stable_fresh G x ∉ G
-  }.
-
-Hint Resolve stable_fresh_spec.
