theories/Alpha/RenameApart_Liveness.v
@@ -1,5 +1,5 @@
 Require Import Util CSet Map LengthEq.
-Require Import Env IL Alpha Fresh Subset1 OptionR.
+Require Import Env IL Alpha StableFresh Subset1 OptionR.
 Require Import Annotation AnnP RenamedApart RenameApart SetOperations Take.
 Require Import LabelsDefined PairwiseDisjoint Liveness Coherence Restrict.
 
