theories/Alpha/RenameApart_VarP.v
@@ -1,0 +1,92 @@
+Require Import Util CSet Var.
+Require Import StableFresh.
+Require Import IL RenameApart.
+
+Inductive var_P (P:var -> Prop)
+  : stmt -> Prop :=
+| VarPOpr x b e
+  :  var_P P b
+     -> P x
+     -> For_all P (Exp.freeVars e)
+     -> var_P P (stmtLet x e b)
+| VarPIf e b1 b2
+  :  For_all P (Op.freeVars e)
+     -> var_P P b1
+     -> var_P P b2
+     -> var_P P (stmtIf e b1 b2)
+| VarPGoto l Y
+  : For_all P (list_union (Op.freeVars ⊝ Y))
+    -> var_P P (stmtApp l Y)
+| VarPReturn e
+  : For_all P (Op.freeVars e)
+    -> var_P P (stmtReturn e)
+| VarPLet F b
+  : (forall n Zs, get F n Zs -> var_P P (snd Zs))
+    -> (forall n Zs, get F n Zs -> For_all P (of_list (fst Zs)))
+    -> var_P P b
+    -> var_P P (stmtFun F b).
+
+
+Instance For_all_P_Equal X `{OrderedType X} (P:X->Prop) `{Proper _ (_eq ==> iff) P}
+  : Proper (Equal ==> iff) (For_all P).
+Proof.
+  unfold Proper, respectful, For_all; split; intros; eapply H2; cset_tac.
+Qed.
+
+Instance For_all_P_Subset X `{OrderedType X} (P:X->Prop) `{Proper _ (_eq ==> iff) P}
+  : Proper (Subset ==> flip impl) (For_all P).
+Proof.
+  unfold Proper, respectful, For_all, flip, impl; intros; eapply H2; eauto.
+Qed.
+
+Lemma renameApart_var_P (fresh:StableFresh) (P:var -> Prop) (ϱ:env var) G s
+      (freshP:forall x G, P (fresh G x))
+      (ren:forall x, x ∈ freeVars s -> P (ϱ x))
+  : var_P P (snd (renameApart' fresh ϱ G s)).
+Proof.
+  revert ϱ G ren.
+  sind s; intros; destruct s; simpl;
+    repeat let_pair_case_eq; repeat simpl_pair_eqs; subst; simpl in *.
+  - econstructor; eauto.
+    + eapply IH; eauto.
+      intros; lud; eauto. eapply ren. cset_tac.
+    + rewrite freeVars_renameExp. unfold lookup_set.
+      hnf; intros. cset_tac.
+  - econstructor; eauto.
+    + rewrite rename_op_freeVars; eauto. unfold lookup_set.
+      hnf; intros. cset_tac.
+    + eapply IH; eauto. cset_tac.
+    + eapply IH; eauto. cset_tac.
+  - econstructor.
+    rewrite freeVars_rename_op_list. unfold lookup_set.
+    hnf; intros. cset_tac.
+  - econstructor.
+    rewrite rename_op_freeVars; eauto. unfold lookup_set.
+    hnf; intros. cset_tac.
+  - econstructor; eauto.
+    + intros. inv_get.
+      edestruct get_fst_renameApartF as [? [? ?]]; eauto; dcr; subst.
+      destruct Zs as [Z s']; simpl in *; subst.
+      eapply IH; eauto.
+      intros. decide (x ∈ of_list (fst x0)).
+      * edestruct update_with_list_lookup_in_list; try eapply i; dcr.
+        Focus 2.
+        rewrite H11.
+        exploit fresh_list_stable_get; try eapply H10; eauto; dcr.
+        subst. get_functional. eapply freshP; eauto.
+        eauto with len.
+      * rewrite lookup_set_update_not_in_Z; eauto.
+        eapply ren.
+        eapply incl_left.
+        eapply incl_list_union; [| reflexivity|]; eauto.
+        cset_tac.
+    + intros.
+      intros. inv_get.
+      edestruct get_fst_renameApartF as [? [? ?]]; eauto; dcr; subst.
+      destruct Zs as [Z s']; simpl in *; subst.
+      hnf; intros.
+      eapply fresh_list_stable_In in H0; dcr; subst.
+      eapply freshP.
+    + eapply IH; eauto.
+      cset_tac.
+Qed.
