theories/Infra/StableFresh.v
@@ -1,0 +1,97 @@
+Require Import Nat CSet Take.
+
+Record StableFresh :=
+  {
+    stable_fresh :> set nat -> nat -> nat;
+    stable_fresh_spec : forall G x, stable_fresh G x ∉ G;
+    stable_fresh_ext : forall G G', G [=] G' -> forall x, stable_fresh G x = stable_fresh G' x
+  }.
+
+Hint Resolve stable_fresh_spec stable_fresh_ext.
+
+Section FreshListStable.
+
+  Variable fresh : StableFresh.
+
+  Fixpoint fresh_list_stable (G:set nat) (xl:list nat) : list nat :=
+    match xl with
+      | nil => nil
+      | x::xl => let y := fresh G x in y::fresh_list_stable {y;G} xl
+    end.
+
+  Lemma fresh_list_stable_length (G:set nat) xl
+  : length (fresh_list_stable G xl) = length xl.
+  Proof.
+    general induction xl; eauto. simpl. f_equal; eauto.
+  Qed.
+
+  Definition fresh_set_stable (G:set nat) L : set nat :=
+    of_list (fresh_list_stable G L).
+
+  Lemma fresh_list_stable_spec
+    : forall (G:set nat) L, disj (of_list (fresh_list_stable G L)) G.
+  Proof.
+    intros. general induction L; simpl; intros; eauto.
+    - hnf; intros. cset_tac'.
+      + eapply stable_fresh_spec in H0; eauto.
+      + eapply IHL; eauto; cset_tac.
+  Qed.
+
+  Lemma fresh_set_stable_spec
+  : forall (G:set nat) L, disj (fresh_set_stable G L) G.
+  Proof.
+    eapply fresh_list_stable_spec.
+  Qed.
+
+  Lemma fresh_list_stable_nodup (G: set nat) L
+    : NoDupA eq (fresh_list_stable G L).
+  Proof.
+    general induction L; simpl; eauto.
+    econstructor; eauto. intro.
+    eapply fresh_list_stable_spec.
+    eapply InA_in. eapply H.
+    cset_tac; eauto.
+  Qed.
+
+End FreshListStable.
+
+Lemma fresh_list_stable_ext n G G' (f:StableFresh)
+  : (forall x G G', G [=] G' -> f G x = f G' x)
+    -> G [=] G'
+    -> fresh_list_stable f G n = fresh_list_stable f G' n.
+Proof.
+  intros EXT EQ. general induction n; simpl.
+  - reflexivity.
+  - f_equal; eauto.
+    eapply IHn; eauto.
+    erewrite EXT, EQ; eauto; reflexivity.
+Qed.
+
+Lemma fresh_list_stable_get (fresh : StableFresh) (G: set nat) L x n
+  : get (fresh_list_stable fresh G L) n x
+    -> exists y, get L n y /\
+           x = fresh (of_list (take n (fresh_list_stable fresh G L)) ∪ G) y.
+Proof.
+  intros Get. general induction L; simpl in *.
+  - isabsurd.
+  - inv Get.
+    + simpl. erewrite stable_fresh_ext; eauto.
+      eexists; split; eauto with get. clear; cset_tac.
+    + edestruct IHL; eauto; dcr; subst.
+      eexists; split; eauto using get.
+      simpl. eapply stable_fresh_ext. clear; cset_tac.
+Qed.
+
+Lemma fresh_list_stable_In (fresh : StableFresh) (G: set nat) L x
+  : x ∈ of_list (fresh_list_stable fresh G L)
+    -> exists y G', y ∈ of_list L /\
+           x = fresh G' y /\ G ⊆ G'.
+Proof.
+  intros Get.
+  eapply of_list_get_first in Get; eauto; dcr.
+  eapply fresh_list_stable_get in H; dcr; subst.
+  cset_tac'. do 2 eexists; split; eauto.
+  eapply get_in_of_list; eauto.
+Qed.
+
+Hint Resolve fresh_list_stable_length : len.
