theories/Liveness/Liveness.v
@@ -153,53 +153,6 @@ Proof.
       eauto with cset.
 Qed.
 
-(*
-(** ** Liveness is stable under renaming *)
-
-Lemma live_rename_sound i ZL Lv s an (ϱ:env var)
-: live_sound i ZL Lv s an
-  -> live_sound i (lookup_list ϱ ⊝ ZL) (lookup_set ϱ ⊝ Lv) (rename ϱ s) (mapAnn (lookup_set ϱ) an).
-Proof.
-  intros. general induction H; simpl.
-  - econstructor; eauto using live_exp_rename_sound.
-    + rewrite getAnn_mapAnn.
-      rewrite <- lookup_set_singleton'; eauto.
-      rewrite lookup_set_minus_incl; eauto with cset.
-    + rewrite getAnn_mapAnn.
-      eapply lookup_set_spec; eauto.
-  - econstructor; eauto using live_op_rename_sound.
-    + rewrite getAnn_mapAnn. eapply lookup_set_incl; eauto.
-    + rewrite getAnn_mapAnn. eapply lookup_set_incl; eauto.
-  - econstructor; eauto with len.
-    + cases; eauto.
-      rewrite of_list_lookup_list; eauto.
-      etransitivity. eapply lookup_set_minus_incl; eauto.
-      eapply lookup_set_incl; eauto.
-    + intros; inv_get; eauto using live_op_rename_sound.
-  - econstructor; eauto using live_op_rename_sound.
-  - econstructor; eauto; try rewrite getAnn_mapAnn; eauto with cset len.
-    + repeat rewrite map_map; simpl. rewrite <- map_map.
-      rewrite <- map_app.
-      setoid_rewrite getAnn_mapAnn.
-      setoid_rewrite <- map_map at 3. rewrite <- map_app. eauto.
-    + intros; inv_get. simpl.
-      repeat rewrite map_map; simpl. rewrite <- map_map.
-      rewrite <- map_app.
-      setoid_rewrite getAnn_mapAnn.
-      setoid_rewrite <- map_map at 3. rewrite <- map_app. eauto.
-    + intros; inv_get; simpl.
-      exploit H3; eauto with cset; dcr.
-      split.
-      * rewrite of_list_lookup_list; eauto.
-        rewrite getAnn_mapAnn.
-        eapply lookup_set_incl; eauto.
-      * cases; eauto.
-        rewrite getAnn_mapAnn.
-        rewrite of_list_lookup_list; eauto.
-        rewrite lookup_set_minus_incl; eauto with cset.
-Qed.
- *)
-
 Lemma adapt_premise F als lv
 : (forall (n : nat) (Zs : params * stmt) (a : ann ⦃nat⦄),
    get F n Zs ->
